Added pattern matching for lists and removed their polymorphism.

STLC_SuccNat/Lifted_STLC_SuccNat.v
@@ -7,13 +7,13 @@ Require Import Presence_Conditions.
 Inductive ty' : Type :=
   | Arrow' : ty' -> ty' -> ty'
   | Nat' : ty'
-  | List' : ty' -> ty'.
+  | NatList' : ty'.
 
 Fixpoint lift_ty (T : ty) : ty' :=
   match T with
     | Nat => Nat'
     | Arrow T1 T2 => Arrow' (lift_ty T1) (lift_ty T2)
-    | List T => List' (lift_ty T)
+    | NatList => NatList'
   end.
 
 Definition nat' := variational_value nat.
@@ -26,8 +26,9 @@ Inductive tm' :=
   | const' : nat' -> tm'
   | succ' : tm' -> tm'
 
-  | nil' : ty' -> tm'
-  | cons' : tm' -> tm' -> tm'.
+  | nil' :  tm'
+  | cons' : tm' -> tm' -> tm'
+  | case' : tm' -> tm' -> string -> string -> tm' -> tm'.
 
 Fixpoint lift (t:tm) : tm':=
   match t with
@@ -38,14 +39,15 @@ Fixpoint lift (t:tm) : tm':=
   | const n => (const' [(n, pc_True)])
   | succ t => (succ' (lift t))
 
-  | nil T => (nil' (lift_ty T))
+  | nil => nil'
   | cons t1 t2 => cons' (lift t1) (lift t2)
+  | case t1 tnil x y tcons => case' (lift t1) (lift tnil) x y (lift tcons)
   end.
 
 Inductive value' : tm' -> Prop :=
   | v_abs' : forall x T' t', value' (abs' x T' t')
   | v_nat' : forall n', value' (const' n')
-  | v_lnil' : forall T', value' (nil' T')
+  | v_lnil' : value' nil'
   | v_lcons' : forall v1' v2', value' v1' -> value' v2' -> value' (cons' v1' v2').
 
 Fixpoint subst' (x:string) (s' t': tm'): tm' :=
@@ -57,8 +59,10 @@ Fixpoint subst' (x:string) (s' t': tm'): tm' :=
   | const' _ => t'
   | succ' t1' => succ' (subst' x s' t1')
 
-  | nil' T' => nil' T'
+  | nil' => nil'
   | cons' t1' t2' => cons' (subst' x s' t1') (subst' x s' t2')
+  | case' t1' t2' y z t3' => case' (subst' x s' t1') (subst' x s' t2') y z
+                                        (if (orb (eqb x y) (eqb x z)) then t3' else (subst' x s' t3'))
   end.
 
 Inductive step': tm' -> tm' -> Prop :=
@@ -86,7 +90,16 @@ Inductive step': tm' -> tm' -> Prop :=
   | ST_Cons2': forall v1' t2' t3',
     value' v1' ->
     step' t2' t3' ->
-    step' (cons' v1' t2') (cons' v1' t3').
+    step' (cons' v1' t2') (cons' v1' t3')
+  | ST_Case1': forall x y t1' t2' tnil' tcons',
+    step' t1' t2' ->
+    step' (case' t1' tnil' x y tcons') (case' t2' tnil' x y tcons')
+  | ST_CaseNil': forall x y tnil' tcons',
+    step' (case' nil' tnil' x y tcons') tnil'
+  | ST_CaseCons': forall x y vh' vt' tnil' tcons',
+    value' vh' ->
+    value' vt' ->
+    step' (case' (cons' vh' vt') tnil' x y tcons') (subst' y vt' (subst' x vh' tcons')).
 
 Definition step'_normal_form_of t1' t2':=
   (multi step' t1' t2' /\ normal_form step' t2').
@@ -115,12 +128,17 @@ Inductive has_type': context' -> tm' -> ty' -> Prop :=
     has_type' Gamma' t' Nat' ->
       has_type' Gamma' (succ' t') Nat'
 
-  | T_Nil' : forall Gamma' T',
-    has_type' Gamma' (nil' T') (List' T')
-  | T_Cons' : forall Gamma' t1' t2' T',
-    has_type' Gamma' t1' T' ->
-    has_type' Gamma' t2' (List' T') ->
-      has_type' Gamma' (cons' t1' t2') (List' T').
+  | T_Nil' : forall Gamma',
+    has_type' Gamma' nil' NatList'
+  | T_Cons' : forall Gamma' t1' t2',
+    has_type' Gamma' t1' Nat' ->
+    has_type' Gamma' t2' NatList' ->
+      has_type' Gamma' (cons' t1' t2') NatList'
+  | T_Case' : forall Gamma' x y T' t1' tnil' tcons',
+    has_type' Gamma' t1' NatList' ->
+    has_type' Gamma' tnil' T' ->
+    has_type' (x |-> Nat'; y |-> NatList'; Gamma') tcons' T' ->
+    has_type' Gamma' (case' t1' tnil' x y tcons') T'.
 
 (* Typing Theorems *)
 Lemma weakening': forall Gamma1' Gamma2' t' T',
@@ -164,6 +182,21 @@ Proof.
   exists x, t1'. reflexivity.
 Qed.
 
+(*TODO: Is this right?*)
+Lemma canonical_forms_list' : forall t',
+  has_type' empty t' NatList' ->
+  value' t' ->
+    t' = nil' \/
+    (exists v1' v2',
+      value' v1' /\ value' v2' /\ t' = (cons' v1' v2')).
+Proof.
+  intros t HT Hv.
+  destruct Hv; inversion HT; subst; eauto 7.
+(*- auto.
+  - right. exists v1, v2.
+    split; [auto|split;auto]. *)
+Qed.
+
 Theorem progress' : forall t1' T',
   has_type' empty t1' T' ->
     value' t1' \/ exists t2', step' t1' t2'.
@@ -191,6 +224,14 @@ Proof.
         eexists; eauto using ST_Cons2'.
     + right. unfold_exists.
       eexists; eauto using ST_Cons1'.
+  - destruct IHHt1; auto; right.
+    + destruct t1';
+        try solve_by_inverts 1; eexists.
+        * apply ST_CaseNil'.
+        * inversion H; subst.
+          eapply ST_CaseCons'; auto.
+    + unfold_exists. eexists.
+      constructor. eauto.
 Qed.
 
 Lemma substitution_preserves_typing': forall Gamma' x U' t' v' T',
@@ -203,7 +244,7 @@ Proof.
   induction t'; intros T' Gamma' H;
     inversion H; clear H; subst; simpl; eauto;
     try (econstructor; eauto);
-    destruct (eqb_spec x s); subst; try (constructor).
+    destruct (eqb_spec x s); subst; simpl; try (constructor).
     + rewrite update_eq in H2.
       injection H2 as H2; subst.
       apply weakening_empty'. assumption.
@@ -211,6 +252,20 @@ Proof.
     + rewrite update_shadow in H5. assumption.
     + apply IHt'. eapply update_permute in n.
       rewrite n in H5. assumption.
+    + destruct (eqb_spec s s0); subst.
+      * repeat rewrite update_shadow in H9.
+        rewrite update_shadow. assumption.
+      * rewrite update_permute in H9; auto.
+        rewrite update_shadow in H9.
+        rewrite update_permute; auto.
+    + destruct (eqb_spec x s0); subst.
+      * rewrite update_shadow in H9. assumption.
+      * apply IHt'3. assert (
+          (x) |-> U'; (s) |-> Nat'; (s0) |-> NatList'; Gamma' =
+          (s) |-> Nat'; (s0) |-> NatList'; (x) |-> U'; Gamma').
+        { rewrite update_permute; auto. f_equal.
+          rewrite update_permute; auto. }
+        rewrite H. assumption.
 Qed.
 
 Theorem preservation': forall t1' t2' T',
@@ -225,9 +280,12 @@ Proof.
     inversion H0; subst;
       try (econstructor; eauto).
   apply (T_App' _ _ _ _ _ Ht1) in Ht2.
-  eapply substitution_preserves_typing';
+  - eapply substitution_preserves_typing';
     inversion Ht2; inversion H4; subst;
     eassumption.
+  - assumption.
+  - inversion Ht1; subst.
+    repeat eapply substitution_preserves_typing'; eauto.
 Qed.
 
 Lemma preservation'_multi: forall t1' t2' T',
@@ -301,7 +359,11 @@ Ltac value'_no_step :=
 	match goal with
 	| [ H1: value' ?t, H2: step' ?t  _ |- _ ] =>
 		exfalso; apply value'_is_nf in H1 as [_ H1]; eauto
-	end.
+	| [ H1: value' ?t1, H2: value' ?t2, H3: step' (cons' ?t1 ?t2) _ |- _] =>
+    inversion H3; subst; exfalso;
+             apply value'_is_nf in H1 as [_ H1];
+             apply value'_is_nf in H2 as [_ H2]; eauto
+  end.
 
 Theorem determinism' : forall t1' t2' t3',
   step' t1' t2' -> step' t1' t3' -> t2' = t3'.
@@ -383,6 +445,16 @@ Proof.
     eapply T_Cons'.
     + apply IHH_type1. exact H_equiv.
     + apply IHH_type2. exact H_equiv.
+  - (* T_Case' *)
+    eapply T_Case'.
+    + apply IHH_type1. assumption.
+    + apply IHH_type2. assumption.
+    + apply IHH_type3. intro z.
+      unfold update.
+      destruct (eqb x z) eqn:Heq;
+        unfold t_update;
+        rewrite Heq; auto.
+      destruct (eqb y z) eqn:Heq0; auto.
 Qed.
 
 Lemma lift_context_update : forall (Gamma : partial_map ty) x T y,
@@ -411,6 +483,15 @@ Proof.
   - apply has_type'_lookup_equiv with (lift_context (x |-> T2; Gamma)).
     + intro y. apply lift_context_update.
     + exact IHhas_type.
+  - apply has_type'_lookup_equiv with (lift_context (x) |-> Nat; (y) |-> NatList; Gamma).
+    + intro z. repeat rewrite lift_context_update.
+      destruct (eqb_spec x z), (eqb_spec y z);
+        subst; unfold update;
+        try (rewrite t_update_eq; auto);
+        try (rewrite t_update_neq; auto).
+        rewrite t_update_eq; auto.
+        rewrite t_update_neq; auto.
+    + exact IHhas_type3.
 Qed.
 
 Lemma lifting_types_empty: forall t T,
@@ -453,6 +534,11 @@ Proof.
     rewrite IHbody1.
     rewrite IHbody2.
     reflexivity.
+  - (* Case *)
+    destruct (eqb_spec x s), (eqb_spec x s0);
+    rewrite IHbody1, IHbody2;
+     simpl; auto.
+    rewrite IHbody3; reflexivity.
 Qed.
 
 Lemma value_value': forall v,
@@ -492,6 +578,14 @@ Proof.
       apply ST_Cons2';
         try (apply value_value' in H1);
         assumption.
+  - inversion Hstep; subst; simpl.
+    + apply IHt1_1 in H5.
+      apply ST_Case1'.
+      assumption.
+    + apply ST_CaseNil'.
+    + repeat rewrite lift_subst_subst'_lift.
+      apply ST_CaseCons';
+        auto using value_value'.
 Qed.
 
 Lemma mstep_mstep': forall t1 t2,
